agda/nat_def.agda
@@ -1,0 +1,90 @@
+module nat_def where
+
+-- Constructor for natural numbers.
+data ℕ : Set where
+  zero : ℕ
+  suc  : ℕ → ℕ
+
+{-# BUILTIN NATURAL ℕ #-}
+
+seven = suc (suc (suc (suc (suc (suc (suc 0))))))
+
+import Relation.Binary.PropositionalEquality as Eq
+open Eq using (_≡_; refl)
+open Eq.≡-Reasoning using (begin_; _≡⟨⟩_; _∎)
+
+_+_ : ℕ → ℕ → ℕ
+0 + n = n
+suc m + n = suc (m + n)
+
+_*_ : ℕ → ℕ → ℕ
+0 * n = 0
+suc m * n = n + (m * n)
+
+_-_ : ℕ → ℕ → ℕ
+n - 0 = 0
+0 - n = 0
+suc m - suc n = m - n
+
+five = 8 - 3
+another_five = 7 - 2
+
+_ =
+  begin
+    2 * 3
+  ≡⟨⟩ 
+    3 + (1 * 3)
+  ≡⟨⟩ 
+    3 + (3 + (0 * 3))
+  ≡⟨⟩ 
+    3 + (3 + 0)
+  ≡⟨⟩ 
+    6
+  ∎
+
+_ =
+  begin
+    3 * 4
+  ≡⟨⟩
+    4 + (2 * 4)
+  ≡⟨⟩
+    4 + (4 + (1 * 4))
+  ≡⟨⟩
+    4 + (4 + (4 + (0 * 4)))
+  ≡⟨⟩
+    (4 + (4 + (4 + 0)))
+  ≡⟨⟩
+    (4 + (4 + 4))
+  ≡⟨⟩
+    4 + 8
+  ≡⟨⟩
+    12
+  ∎
+
+_^_ : ℕ → ℕ → ℕ
+n ^ 0 = 1
+n ^ (suc m) = n * (n ^ m)
+
+_ =
+  begin
+    3 ^ 4
+  ≡⟨⟩
+    3 * (3 ^ 3)
+  ≡⟨⟩
+    3 * (3 * (3 ^ 2))
+  ≡⟨⟩
+    3 * (3 * (3 * (3 ^ 1)))
+  ≡⟨⟩
+    3 * (3 * (3 * (3 * (3 ^ 0))))
+  ≡⟨⟩
+    3 * (3 * (3 * (3 * 1)))
+  ≡⟨⟩
+    3 * (3 * (3 * 3))
+  ≡⟨⟩
+    3 * (3 * 9)
+  ≡⟨⟩
+    3 * 27
+  ≡⟨⟩
+    81
+  ∎
+
