agda/nat_ind.agda
@@ -1,0 +1,84 @@
+
+import Relation.Binary.PropositionalEquality as Eq
+open Eq using (_≡_; refl; cong; sym)
+open Eq.≡-Reasoning using (begin_; _≡⟨⟩_; step-≡; _∎)
+open import Data.Nat using (ℕ; zero; suc; _+_; _*_; _∸_;_^_)
++-assoc : ∀ (m n p : ℕ) → (m + n) + p ≡ m + (n + p)
++-assoc 0 n p =
+  begin
+    (0 + n) + p
+  ≡⟨⟩
+    n + p
+  ≡⟨⟩
+    0 + (n + p)
+  ∎
++-assoc (suc m) n p =
+  begin
+    (suc m + n) + p
+  ≡⟨⟩
+    suc (m + n) + p
+  ≡⟨⟩
+    suc ((m + n) + p)
+  ≡⟨ cong suc (+-assoc m n p) ⟩
+    suc (m + (n + p))
+  ≡⟨⟩
+    suc m + (n + p)
+  ∎
+
++-zero-elim : ∀ (n : ℕ) → n + 0 ≡ n
++-zero-elim 0 =
+  begin
+    0 + 0
+  ≡⟨⟩
+    0
+  ∎
++-zero-elim (suc n) =
+  begin
+    suc n + 0
+  ≡⟨⟩
+    suc (n + 0)
+  ≡⟨ cong suc (+-zero-elim n) ⟩
+    suc n
+  ∎
+
++-right-suc : ∀ (m n : ℕ) -> m + suc n ≡ suc (m + n) 
++-right-suc 0 n =
+  begin
+    0 + suc n
+  ≡⟨⟩
+    suc n
+  ≡⟨⟩
+    suc (0 + n)
+  ∎
+
++-right-suc (suc m) n =
+  begin
+    suc m + suc n
+  ≡⟨⟩
+    suc (m + suc n)
+  ≡⟨ cong suc (+-right-suc m n) ⟩
+    suc (suc (m + n))
+  ≡⟨⟩
+    suc (suc m + n)
+  ∎
+
++-comm : ∀ (m n : ℕ) -> m + n ≡ n + m
++-comm m 0 =
+  begin
+    m + 0
+  ≡⟨ +-zero-elim m ⟩
+    m
+  ≡⟨⟩
+    0 + m
+  ∎
+
++-comm m (suc n) =
+  begin
+    m + suc n
+  ≡⟨ +-right-suc m n ⟩
+    suc (m + n)
+  ≡⟨ cong suc (+-comm m n) ⟩
+    suc (n + m)
+  ≡⟨⟩
+    suc n + m
+  ∎
